committing for ask arthur

semantics/proofs_working.v
@@ -350,20 +350,28 @@ Lemma cp_const {N01 N02 V01 V02 c01 c02 N1 N2 V1 V2 c1 c2 O W} :
   checkpoint \notin O ->
   N01 = N02 /\ V01 = V02 /\ c01 = c02. Admitted.
 
+      Inductive same_mem11 {N0 Nstart Nvar Nc V c N Nend Vend cend O W}:
+        (current_init_pt N0 V c Nstart Nvar Nc) ->
+        trace_i ((N0, V, c), N, V, c) ((N0, V, c), Nend, Vend, cend) O W ->
+        Prop :=
+        Same_Mem11: forall(H: current_init_pt N0 V c Nstart Nvar Nc)
+(T: trace_i ((N0, V, c), N, V, c) ((N0, V, c), Nend, Vend, cend) O W),
+          Nvar = N -> same_mem11 H T.
 
     Lemma eleven: forall{N0 N1 Nmid Nend N2: nvmem} {V Vmid Vend: vmem} {c cmid cend: command}
-                   {O1 Orem: obseq} {W1 Wrem: the_write_stuff},
-        trace_i ((N0, V, c), N1, V, c) ((N0, V, c), Nmid, Vmid, cmid) O1 W1 ->
+                   {O1 Orem: obseq} {W1 Wrem: the_write_stuff} 
+                   (T: trace_i ((N0, V, c), N1, V, c) ((N0, V, c), Nmid, Vmid, cmid) O1 W1)
+             (H: current_init_pt N0 V c N1 N1 N2),
              (checkpoint \notin O1) ->
              subset_nvm N0 N1 ->
              subset_nvm N0 N2 ->
-             current_init_pt N0 V c N1 N1 N2 ->
              WARok (getdomain N0) [::] [::] c ->
              trace_i ((N0, V, c), Nmid, Vmid, cmid) ((N0, V, c), Nend, Vend, cend) Orem Wrem ->
              (* Sigma -> Sigma'
 configs can always make progress assumption*)
              (checkpoint \notin Orem) ->
              (reboot \notin Orem) ->
+             same_mem11 H T ->
              ((cend = Ins skip) \/ exists(w: warvars) (cend2: command), cend = (incheckpoint w);; cend2) ->
              (exists(O2: obseq) (sigma: context) (Wc:
                                             the_write_stuff),
@@ -381,12 +389,16 @@ configs can always make progress assumption*)
              (*same obs, write as "intermittent" execution*)
              (O1 ++ Orem <=m O2 ++ Orem)).
       intros.
-      move: H0 H1 H2 H3 H4 H5 H6 H7 H8.
+      move: H H0 H1 H2 H3 H4 H5 H6 H7 H8.
       move: Wrem Orem cend Vend Nend N2.
-      apply trace_convert in H.
-      induction H; intros.
+      assert (trace_i (N0, V, c, N1, V, c)
+                      (N0, V, c, Nmid, Vmid, cmid) O1 W1) as T1.
+      apply T.
+      (*ask arthur what the hell is this*)
+      apply trace_convert in T1.
+      induction T1; intros.
       2: {
-        pose proof (cp_const H9 H10) as [eq1 [eq2 eq3] ]. subst.
+        pose proof (cp_const H8 H9) as [eq1 [eq2 eq3] ]. subst.
         suffices: (exists O3 sigma Wc,
                trace_c (N3, V, c) sigma O3 Wc /\
                       is_true (checkpoint \notin O3) /\
@@ -404,8 +416,8 @@ configs can always make progress assumption*)
       repeat (try split); try assumption.
       destruct3 sigma Ns Vs cs.
       pose proof (obseq_readobs Hc1 Hc2) as [o3 Ho3].
-      pose proof (obseq_readobs Hc4 H10) as [o4 Ho4].
-      pose proof (obseq_readobs H H1) as [o1 Ho1].
+      pose proof (obseq_readobs Hc4 H9) as [o4 Ho4].
+      pose proof (obseq_readobs H H0) as [o1 Ho1].
       (*dont think obseq_readobs is actually true
        because the trace doesnt append consecutive read observations together*
       why do i even need the above
@@ -437,7 +449,13 @@ configs can always make progress assumption*)
       (*consider having two directions for trace_Convertso that
        you can combine this*)
       apply trace_convert in Hi. apply trace_convert in Tendci.
-                  pose proof (eleven_bc Hi H31 Ho1 H3 H6 H7 H8
+      (*prop which forces N1 from
+current init and Ns2 to be the same
+       *)
+
+inversion H11.
+
+                  pose proof (eleven_bc Hi H31 Ho1 H2 H6 H7 H8
                            Tendci 
                             Hcend1 Hoend
                             Hcend2)
